Tidy

Coxeter/StrongExchange.lean
@@ -3,8 +3,25 @@ import Coxeter.PermutationRepresentation
 /-!
 # Strong Exchange
 
-This file proves the strong exchange property of Coxeter groups and friends.
+This file proves the strong exchange property and friends of Coxeter groups.
 -/
+
+namespace List
+
+theorem drop_eraseIdx {α : Type*} (l : List α) (i j : ℕ) :
+  (drop i l).eraseIdx j = drop i (l.eraseIdx (i + j)) := by
+  revert l
+  induction i with
+  | zero => simp
+  | succ i ih =>
+      intro l
+      cases l with
+      | nil => simp
+      | cons a as =>
+          rw [add_right_comm]
+          apply ih
+
+end List
 
 namespace Coxeter
 
@@ -15,9 +32,9 @@ variable {W : Type*} [CoxeterGroup W]
 open Classical in
 /-- Bjorner--Brenti Corollary 1.4.4 (a) implies (c) -/
 theorem mem_leftInvSeq_of_isLeftInversion
-  {ω : List (B W)} {t : W} (ht : cs.IsReflection t) (h : cs.IsLeftInversion (cs.wordProd ω) t) :
+  {ω : List (B W)} {t : W} (h : cs.IsLeftInversion (cs.wordProd ω) t) :
   t ∈ cs.leftInvSeq ω := by
-  have hrw := eta_eq_one_iff (cs.wordProd ω) t ht
+  have hrw := eta_eq_one_iff (cs.wordProd ω) t h.1
   rw [IsLeftInversion, ←hrw, eta_spec] at h
   have h2 : 0 < count t (cs.leftInvSeq ω) := by
     rw [pos_iff_ne_zero]
@@ -34,15 +51,15 @@ theorem isLeftInversion_iff_mem_leftInvSeq
   cs.IsLeftInversion (cs.wordProd ω) t ↔ t ∈ cs.leftInvSeq ω := by
   constructor
   · intro h
-    exact mem_leftInvSeq_of_isLeftInversion h.1 h
+    exact mem_leftInvSeq_of_isLeftInversion h
   · exact cs.isLeftInversion_of_mem_leftInvSeq hω
 
 open Classical in
 /-- Bjorner--Brenti Theorem 1.4.3 -/
 theorem strong_exchange
-  {ω : List (B W)} {t : W} (ht : cs.IsReflection t) (h : cs.IsLeftInversion (cs.wordProd ω) t) :
+  {ω : List (B W)} {t : W} (h : cs.IsLeftInversion (cs.wordProd ω) t) :
   ∃ i < ω.length, t * cs.wordProd ω = cs.wordProd (ω.eraseIdx i) := by
-  have h2 := mem_leftInvSeq_of_isLeftInversion ht h
+  have h2 := mem_leftInvSeq_of_isLeftInversion h
   rw [mem_iff_get] at h2
   let ⟨i, hi⟩ := h2
   exists i
@@ -51,60 +68,65 @@ theorem strong_exchange
     exact i.prop
   · rw [←hi, ←getD_leftInvSeq_mul_wordProd, getD_eq_get]
 
-open Classical in
-theorem leftInversionSet_eq {ω : List (B W)} (hω : cs.IsReduced ω) :
-  setOf (cs.IsLeftInversion (cs.wordProd ω)) = (cs.leftInvSeq ω).toFinset := by
-  ext t
-  simp only [Set.mem_setOf_eq, coe_toFinset]
-  exact isLeftInversion_iff_mem_leftInvSeq _ hω
+theorem exchange_property
+  {ω : List (B W)} {i : B W} (h : cs.IsLeftDescent (cs.wordProd ω) i) :
+  ∃ j < ω.length, cs.simple i * cs.wordProd ω = cs.wordProd (ω.eraseIdx j) :=
+  strong_exchange ⟨cs.isReflection_simple i, h⟩
 
-theorem finite_of_isLeftInversion (w : W) : Set.Finite (cs.IsLeftInversion w) := by
-  let ⟨ω, ⟨hω1, hω2⟩⟩ := cs.exists_reduced_word w
-  subst hω2
-  rw [Eq.comm] at hω1
-  change cs.IsReduced ω at hω1
-  change Finite (setOf (cs.IsLeftInversion (cs.wordProd ω)))
-  rw [leftInversionSet_eq hω1]
-  apply finite_toSet
+open Classical in
+def equivIsLeftInversion (ω : List (B W)) (hω : cs.IsReduced ω) :
+  {t : W // cs.IsLeftInversion (cs.wordProd ω) t} ≃ (cs.leftInvSeq ω).toFinset :=
+    Equiv.subtypeEquivRight
+      (fun t => by rw [mem_toFinset]; exact isLeftInversion_iff_mem_leftInvSeq t hω)
+
+open Classical in
+noncomputable instance {w : W} : Fintype {t : W // cs.IsLeftInversion w t} := by
+  have ⟨h1, h2⟩ := choose_spec (cs.exists_reduced_word' w)
+  have h := equivIsLeftInversion (choose (cs.exists_reduced_word' w)) h1
+  rw [←h2] at h
+  exact Fintype.ofEquiv _ h.symm
 
 open Classical in
 /-- Bjorner--Brenti Corollary 1.4.5 -/
 theorem card_of_leftInversionSet (w : W) :
-  Nat.card (setOf (cs.IsLeftInversion w)) = cs.length w := by
-  let ⟨ω, ⟨hω1, hω2⟩⟩ := cs.exists_reduced_word w
+  Fintype.card {t : W // cs.IsLeftInversion w t} = cs.length w := by
+  let ⟨ω, ⟨hω1, hω2⟩⟩ := cs.exists_reduced_word' w
   subst hω2
-  rw [Eq.comm] at hω1
-  change cs.IsReduced ω at hω1
-  rw [Nat.subtype_card (cs.leftInvSeq ω).toFinset]
-  · rw [toFinset_card_of_nodup]
-    · simp only [length_leftInvSeq]
-      exact hω1.symm
-    · exact hω1.nodup_leftInvSeq
-  · simp only [mem_toFinset, Set.mem_setOf_eq]
-    intro x
-    exact (isLeftInversion_iff_mem_leftInvSeq x hω1).symm
+  rw [hω1]
+  trans (cs.leftInvSeq ω).toFinset.card
+  · rw [Fintype.card_congr (equivIsLeftInversion ω hω1)]
+    have h : Fintype.card (cs.leftInvSeq ω).toFinset = (cs.leftInvSeq ω).toFinset.card := by
+      apply Fintype.card_ofFinset ((cs.leftInvSeq ω).toFinset)
+      tauto
+    exact h
+  · rw [toFinset_card_of_nodup (hω1.nodup_leftInvSeq), length_leftInvSeq]
 
-private theorem drop_eraseIdx (l : List (B W)) (i j : ℕ) :
-  (drop i l).eraseIdx j = drop i (l.eraseIdx (i + j)) := by
-  revert l
-  induction i with
-  | zero => simp
-  | succ i ih =>
-      intro l
-      cases l with
-      | nil => simp
-      | cons a as =>
-          rw [add_right_comm]
-          apply ih
+theorem IsReduced_nil (W : Type*) [CoxeterGroup W] : (@cs W).IsReduced [] := by
+  unfold CoxeterSystem.IsReduced
+  rw [wordProd_nil, length_one, length_nil]
+
+theorem not_IsReduced_cons {ω : List (B W)} (i : B W) (hω : cs.IsReduced ω) :
+  ¬ cs.IsReduced (i :: ω) ↔ cs.IsLeftDescent (cs.wordProd ω) i := by
+  unfold CoxeterSystem.IsReduced IsLeftDescent at *
+  rw [hω, wordProd_cons, length_cons]
+  have := cs.length_simple_mul (cs.wordProd ω) i
+  grind
 
 open Classical in
 /-- Bjorner--Brenti Proposition 1.4.7 -/
-theorem deletion_property {ω : List (B W)} (hω : cs.length (cs.wordProd ω) < ω.length) :
+theorem deletion_property {ω : List (B W)} (hω : ¬ cs.IsReduced ω) :
   ∃ i j, i < j ∧ j < ω.length ∧ cs.wordProd ω = cs.wordProd ((ω.eraseIdx j).eraseIdx i) := by
+  have h0 : ω ≠ [] := by
+    intro h
+    subst h
+    have := IsReduced_nil W
+    contradiction
   have h1 : cs.IsReduced (drop ((ω.length - 1) + 1) ω) := by
     rw [Nat.sub_one_add_one]
-    · simp [CoxeterSystem.IsReduced]
-    · grind
+    · rw [drop_length]
+      apply IsReduced_nil
+    · rw [ne_eq, length_eq_zero_iff]
+      exact h0
   have h2 : ∃ i, cs.IsReduced (drop (i + 1) ω) := by
     exists ω.length - 1
   let i := Nat.find h2
@@ -113,33 +135,25 @@ theorem deletion_property {ω : List (B W)} (hω : cs.length (cs.wordProd ω) < 
     cases Nat.eq_zero_or_pos i with
     | inl h =>
         rw [h]
-        unfold CoxeterSystem.IsReduced
-        grind
+        exact hω
     | inr h =>
-        replace h : i ≠ 0 := by grind
+        replace h : i ≠ 0 := Nat.ne_of_gt h
         rw [←Nat.sub_one_add_one h]
         apply Nat.find_min h2
         exact Nat.sub_one_lt h
   have h5 : i < ω.length := by
     rw [Nat.find_lt_iff]
     exists ω.length - 1
-    grind
-  have h6 : cs.length (cs.simple ω[i] * cs.wordProd (drop (i + 1) ω)) + 1
-    = cs.length (cs.wordProd (drop (i + 1) ω)):= by
-    rw [←isLeftDescent_iff]
-    by_contra h
-    rw [not_isLeftDescent_iff, ←wordProd_cons] at h
-    simp only [getElem_cons_drop] at h
-    unfold CoxeterSystem.IsReduced at *
-    grind
-  have h7 : cs.IsLeftInversion (cs.wordProd (drop (i + 1) ω)) (cs.simple ω[i]) := by
     constructor
-    · exact cs.isReflection_simple _
-    · grind
-  let ⟨k, ⟨hk1, hk2⟩⟩ := strong_exchange (cs.isReflection_simple ω[i]) h7
-  exists i
-  exists i + k + 1
-  dsimp at *
+    · apply Nat.sub_one_lt
+      rw [ne_eq, List.length_eq_zero_iff]
+      exact h0
+    · exact h1
+  have h6 : cs.IsLeftDescent (cs.wordProd (drop (i + 1) ω)) ω[i] := by
+    rw [←not_IsReduced_cons ω[i] h3, getElem_cons_drop]
+    exact h4
+  let ⟨k, hk1, hk2⟩ := exchange_property h6
+  exists i, i + k + 1
   apply And.intro (by grind) (And.intro (by grind) _)
   rw [eraseIdx_eq_take_drop_succ, take_eraseIdx_eq_take_of_le _ i (i + k + 1) (by grind)]
   nth_rw 1 [←take_append_drop i ω]
@@ -148,41 +162,24 @@ theorem deletion_property {ω : List (B W)} (hω : cs.length (cs.wordProd ω) < 
   congr
   apply drop_eraseIdx
 
-theorem deletion_property' {ω : List (B W)} (hω : ¬ cs.IsReduced ω) :
-  ∃ i j, i < j ∧ j < ω.length ∧ cs.wordProd ω = cs.wordProd ((ω.eraseIdx j).eraseIdx i) := by
-  apply deletion_property
-  unfold CoxeterSystem.IsReduced at hω
-  have := cs.length_wordProd_le ω
-  grind
-
 /-- Bjorner--Brenti Corollary 1.4.8 (i) -/
 theorem exists_reduced_subword (ω : List (B W)) :
   ∃ (ω' : List (B W)), ω' <+ ω ∧ cs.IsReduced ω' ∧ cs.wordProd ω = cs.wordProd ω' := by
-  revert ω
-  suffices h : ∀ k, ∀ ω : List (B W), ω.length < k →
-    ∃ (ω' : List (B W)), ω' <+ ω ∧ cs.IsReduced ω' ∧ cs.wordProd ω = cs.wordProd ω' from by
-    intro ω
-    apply h (ω.length + 1)
-    simp
-  intro k
-  induction k with
-  | zero => simp
-  | succ k ih =>
-      intro ω h
+  induction ω using Nat.strongRecMeasure List.length with
+  | ind ω ih =>
       cases em (cs.IsReduced ω) with
-      | inl h2 => exists ω
-      | inr h2 =>
-          let ⟨i, j, h3⟩ := deletion_property' h2
-          have ⟨ω', h4⟩ := ih ((ω.eraseIdx j).eraseIdx i) (by grind)
+      | inl h => exists ω
+      | inr h =>
+          let ⟨i, j, _, _, h2⟩ := deletion_property h
+          let ⟨ω', h3, h4, h5⟩ := ih ((ω.eraseIdx j).eraseIdx i) (by grind)
           exists ω'
-          apply And.intro
-          · trans
-            · exact h4.1
-            · trans
-              · apply eraseIdx_sublist
-              · apply eraseIdx_sublist
-          · apply And.intro
-            · exact h4.2.1
-            · grind
+          constructor
+          · calc
+              ω' <+ (ω.eraseIdx j).eraseIdx i := h3
+              _ <+ (ω.eraseIdx j) := eraseIdx_sublist _ _
+              _ <+ ω := eraseIdx_sublist _ _
+          · constructor
+            · exact h4
+            · rw [h2, h5]
 
 end Coxeter
